implement bir_lifting_machinesLib
after the logic definition of a machine dependend record, now a lib for
the ML side is provided. This lead to the extension of the HOL record
with a next state function field.

src/tools/lifter/bir_lifting_machinesLib.sig
@@ -1,0 +1,100 @@
+signature bir_lifting_machinesLib =
+sig
+   include Abbrev
+
+   (***************)
+   (* Some Syntax *)
+   (***************)
+
+   (* record type bir_lifting_machine_rec_t has 3 type arguments. MK and DEST
+      below expect them in the following order:
+
+      - machine state type
+      - size of memory addresses
+      - size of memory values
+   *)
+   val mk_bir_lifting_machine_rec_t_ty   : hol_type * hol_type * hol_type -> hol_type
+   val dest_bir_lifting_machine_rec_t_ty : hol_type -> hol_type * hol_type * hol_type
+   val is_bir_lift_machine_rec_t_ty      : hol_type -> bool
+
+   val bmr_ok_tm   : term
+   val dest_bmr_ok : term -> term
+   val is_bmr_ok   : term -> bool
+   val mk_bmr_ok   : term -> term
+
+   val bmr_rel_tm   : term
+   val dest_bmr_rel : term -> term * term * term
+   val is_bmr_rel   : term -> bool
+   val mk_bmr_rel   : term * term * term -> term
+
+   val bmr_vars_tm   : term
+   val dest_bmr_vars : term -> term
+   val is_bmr_vars   : term -> bool
+   val mk_bmr_vars   : term -> term
+
+   val bmr_temp_vars_tm   : term
+   val dest_bmr_temp_vars : term -> term
+   val is_bmr_temp_vars   : term -> bool
+   val mk_bmr_temp_vars   : term -> term
+
+
+   (******************)
+   (* Simplification *)
+   (******************)
+
+   val bmr_REWRS : thm list
+   val bmr_ss : simpLib.ssfrag
+
+
+   (***************)
+   (* Record Type *)
+   (***************)
+
+   (* for each machine, information is collected in a special record type *)
+   type bmr_rec = {
+      (* The constant for the dest_bir_lifting_machine_rec_t constant *)
+      bmr_const              : term,
+
+      (* A theorem of form "brm_ok r" where r is the constant above *)
+      bmr_ok_thm             : thm,
+
+      (* A theorem evaluating the record constant. All auxilary definitions
+         should be expanded in this theorem. *)
+      bmr_eval_thm           : thm,
+
+      (* evaluation for ``bmr_rel r bs ms`` *)
+      bmr_eval_rel_thm       : thm,
+
+      (* Rewrite for the vars used. Should be of form
+         ``bmr_vars r = [v1; v2; ...]`` *)
+      bmr_eval_vars_thm      : thm,
+
+      (* Rewrite for the temp_vars used. Should be of form
+         ``bmr_temp_vars r = [v1; v2; ...]`` *)
+      bmr_eval_temp_vars_thm : thm,
+
+      (* Some lifting theorem, should be of from
+         |- !bs ms. bmr_rel r bs ms ==>
+                    (bir_is_lifted_exp bs.bst_environ . .) /\
+                    ....
+                    (bir_is_lifted_exp bs.bst_environ . .)
+      *)
+      bmr_lifted_thm         : thm,
+
+      (* Extra lifting theorem useful for this machine type,
+         some special rewrites for e.g. OVERFLOWS ... *)
+      bmr_extra_lifted_thms  : thm list,
+
+      (* A useful ssfrag for this machine type. It should
+         contain e.g. information for deal with the machine state type. *)
+      bmr_extra_ss           : simpLib.ssfrag,
+
+      (* Function evaluationg an instruction given as a hex string and returns
+         a set of step theorems. *)
+      bmr_step_hex           : string -> thm list
+   };
+
+   (* The record for arm8 *)
+   val arm8_bmr_rec : bmr_rec;
+
+end
